Trace equivalence

theories/MP/GLTraceEquiv.v
@@ -18,8 +18,8 @@ Section TraceEquiv.
   Definition step_equiv G P :=
     forall a, (exists G', step a G G') <-> (exists P', lstep a P P').
 
-  Definition trace_equiv G P :=
-    forall a, (exists G', g_lts a G G') <-> (exists P', l_lts a P P').
+  Definition trace_equiv G P : Prop :=
+    forall tr, g_lts tr G <-> l_lts tr P.
 
   Fixpoint add_head p (Q : MsgQ) :=
     match Q with
@@ -31,115 +31,81 @@ Section TraceEquiv.
   Notation msg m := (m.1, inr m.2).
   Notation lab m l := (m.1, inl l).
 
-  Fixpoint merge_mq (Q : MsgQ) (Qs : seq MsgQ) :=
+  Fixpoint merge_mq (Q : MsgQ) (Qs : seq (option MsgQ)) :=
     match Qs with
     | [::] => Some Q
-    | h :: t => if h == Q then merge_mq Q t
+    | h :: t => if h == Some Q then merge_mq Q t
                 else None
     end.
 
-  Definition merge_q (Q : seq MsgQ) :=
+  Definition merge_q (Q : seq (option MsgQ)) :=
     match Q with
     | [::] => Some [::]
-    | h :: t => merge_mq h t
+    | h :: t =>
+      match h with
+      | Some q => merge_mq q t
+      | None => None
+      end
     end.
 
-  Print project.
-
-  Fixpoint q_proj G (p : role) : option (MsgQ * l_ty):=
+  Fixpoint msg_proj G (p : role) : option MsgQ :=
     match G with
-    | rg_end => Some ([::], l_end)
-    | rg_var v => Some ([::], l_var v)
-    | rg_rec G =>
-      match q_proj G p with
-      | Some (Q, P) =>
-        if P == l_var (Rvar.bv 0) then None else Some (Q, l_rec P)
-      | None => None
-      end
-    | rg_msg m G =>
-      match q_proj G p with
-      | Some QP => if m.snd == m.rcv then None
-                   else if m.snd == p
-                        then Some (QP.1, l_send m.rcv m.typ QP.2)
-                        else if m.rcv == p
-                             then Some (QP.1, l_recv m.snd m.typ QP.2)
-                             else Some QP
-      | None => None
-      end
+    | rg_end
+    | rg_var _ => Some [::]
+    | rg_msg _ G
+    | rg_rec G => msg_proj G p
     | rg_rcv m G =>
-      match q_proj G p with
-      | Some QP => if m.snd == m.rcv then None
-                   else if m.snd == p
-                        then Some (add_head (msg m) QP.1, QP.2)
-                        else if m.rcv == p
-                             then Some (QP.1, l_recv m.snd m.typ QP.2)
-                             else Some QP
-      | None => None
-      end
+      if m.snd == p
+      then match msg_proj G p with
+           | Some Q => Some (add_head (msg m) Q)
+           | None => None
+           end
+      else msg_proj G p
     | rg_brn m K =>
-      match
-        (fix q_projK K : option (seq MsgQ * seq (lbl * l_ty)):=
-           match K with
-           | [::] => Some ([::], [::])
-           | lG :: K =>
-             match q_proj lG.2 p, q_projK K with
-             | Some QP, Some QK =>
-                 Some (QP.1 :: QK.1, (lG.1, QP.2) :: QK.2)
-             | _, _ => None
-             end
-           end
-        ) K
-      with
-      | None => None
-      | Some (Q, K) =>
-        match merge_q Q with
-        | None => None
-        | Some Q =>
-          if m.snd == m.rcv then None
-          else if m.snd == p
-               then Some (Q, l_sel m.rcv K)
-               else if m.rcv == p
-                    then Some (Q, l_brn m.snd K)
-                    else match K with
-                         | [::] => None
-                         | h :: t => if all (fun X => h.2 == X.2) t
-                                     then Some (Q, h.2)
-                                     else None
-                         end
-        end
-      end
+      merge_q [seq msg_proj lG.2 p | lG <- K]
     | rg_alt lb m K =>
-      match
-        (fix q_projK K : option (seq MsgQ * seq (lbl * l_ty)):=
-           match K with
-           | [::] => Some ([::], [::])
-           | lG :: K =>
-             match q_proj lG.2 p, q_projK K with
-             | Some QP, Some QK =>
-                 Some (QP.1 :: QK.1, (lG.1, QP.2) :: QK.2)
-             | _, _ => None
-             end
+      if m.snd == p
+      then match merge_q [seq msg_proj lG.2 p | lG <- K] with
+           | Some Q => Some (add_head (lab m lb) Q)
+           | None => None
            end
-        ) K
-      with
-      | None => None
-      | Some (Q, K) =>
-        match merge_q Q, lookup lb K with
-        | Some Q, Some G =>
-          if m.snd == m.rcv then None
-          else if m.snd == p
-               then Some (add_head (lab m lb) Q, G)
-               else if m.rcv == p
-                    then Some (Q, l_brn m.snd K)
-                    else match K with
-                         | [::] => None
-                         | h :: t => if all (fun X => h.2 == X.2) t
-                                     then Some (Q, h.2)
-                                     else None
-                         end
-        | _, _ => None
-        end
-      end
+      else merge_q [seq msg_proj lG.2 p | lG <- K]
+    end.
+
+  Definition project_rcv p r L :=
+    let: (p1, q, t) := p in
+    if p1 == q
+    then None
+    else if q == r
+         then ml_recv p1 t L
+         else L.
+
+  Definition project_alt (p : g_prefix) (r : role) (K : seq (lbl * option l_ty)) :=
+    let: ((p, q), t) := p in
+    if p == q
+    then None
+    else if q == r
+         then ml_brn p K
+         else merge_all K.
+
+  Fixpoint rg_proj G (r : role) : option l_ty :=
+    match G with
+    | rg_end => Some l_end
+    | rg_var v => Some (l_var v)
+    | rg_rec G => let: L := rg_proj G r in
+                  if L == Some (l_var (Rvar.bv 0)) then None else ml_rec L
+    | rg_rcv m G => project_rcv m r (rg_proj G r)
+    | rg_msg m G => project_msg m r (rg_proj G r)
+    | rg_brn p K => let: KL := [seq (X.1, rg_proj X.2 r) | X <- K]
+                    in project_brn p r KL
+    | rg_alt lb p K => let: KL := [seq (X.1, rg_proj X.2 r) | X <- K]
+                       in project_alt p r KL
+    end.
+
+  Definition q_proj G r :=
+    match msg_proj G r, rg_proj G r with
+    | Some Q, Some L => Some (Q, L)
+    | _, _ => None
     end.
 
   Definition q_union (Q1 Q2 : MsgQ) := Q1 ++ Q2.
@@ -156,13 +122,50 @@ Section TraceEquiv.
   Definition q_projection G :=
     q_project G (rg_parts G).
 
+  Lemma g_stequiv G :
+    forall (P : MsgQ * seq (role * l_ty)),
+    q_projection G == Some P ->
+    step_equiv G P.
+  Admitted.
+
+  Lemma g_stproj a G G' :
+    forall (P P' : MsgQ * seq (role * l_ty)),
+    q_projection G == Some P ->
+    step a G G' ->
+    lstep a P P' ->
+    q_projection G' == Some P'.
+  Admitted.
+
+  Lemma qproj_end G :
+    q_projection G == Some ([::], [::]) ->
+    G = rg_end.
+  Admitted.
+
   Lemma g_trequiv G :
     forall (P : MsgQ * seq (role * l_ty)),
     q_projection G == Some P ->
     trace_equiv G P.
   Proof.
-    rewrite /q_projection/trace_equiv.
-  Admitted.
+    move=> P H; rewrite /trace_equiv=> tr; split.
+    - move: tr G P H; cofix Ch; move=> tr G P H; case: tr.
+      + move=> H1; elim/glts_inv: H1=>// _ _ Eq; move: Eq H=><-/=.
+        by rewrite /q_projection/==>/eqP-[<-]; constructor.
+      + move=> a t; elim/glts_inv=>// _ a' t' G0 G' aG tG' [aa' tt' _ {G0}].
+        move: aa' aG=>->aG {a'}.
+        move: tt' tG'=>->tG' {t'}.
+        move: (g_stequiv H) => /(_ a)-[/(_ (ex_intro _ G' aG))-[P' PP'] _].
+        apply: lt_next; [apply: PP'| apply: Ch]; last (by apply: tG').
+        by apply: (g_stproj H aG).
+    - move: tr G P H; cofix Ch; move=> tr G P H; case: tr.
+      + move=> H1; elim/llts_inv: H1=>// _ _ Eq; move: Eq H=><-/=.
+        by move=>/qproj_end->; apply: eg_end.
+      + move=> a t; elim/llts_inv=>// _ a' t' P0 P' aP tP' [aa' tt' _ {P0}].
+        move: aa' aP=>->aP {a'}.
+        move: tt' tP'=>->tP' {t'}.
+        move: (g_stequiv H) => /(_ a)-[_ /(_ (ex_intro _ P' aP))-[G' GG']].
+        apply: eg_trans; [apply: GG'| apply: Ch]; last (by apply: tP').
+        by apply: (g_stproj H GG').
+  Qed.
 
   Lemma rgparts_init G :
     rg_parts (init G) = participants G.
@@ -174,6 +177,23 @@ Section TraceEquiv.
       by apply/Fa_map_eq/forall_member => lG /(Ih lG).
   Qed.
 
+  Lemma msg_project_init G p :
+    msg_proj (init G) p = Some [::].
+  Proof.
+    elim/gty_ind2: G=>// pr K Ih/=; rewrite -map_comp/comp/=.
+    move: Ih; case: K=>[//|[l G] K/= [->]/=].
+    by elim: K=>[//|[l1 G1] K/= Ih [-> /Ih->]].
+  Qed.
+
+  Lemma rg_project_init G p :
+    rg_proj (init G) p = project G p.
+  Proof.
+    elim/gty_ind2: G=>///=.
+    - by move=>G->.
+    - by move=>pr G ->.
+    - move=>pr K /forall_member-Ih; rewrite -map_comp/comp/=; congr project_brn.
+      by apply/Fa_map_eq/forall_member => x xK; move: (Ih x xK)=>->.
+  Qed.
 
   Lemma project_init G P :
     projection G == Some P -> q_projection (init G) = Some ([::], P).
@@ -181,28 +201,10 @@ Section TraceEquiv.
     rewrite /projection/q_projection rgparts_init; elim: (participants G) P.
     - by move=>P /eqP-[<-].
     - move=> a ps Ih/= P.
-      suff: forall L, project G a == Some L ->
-                      q_proj (init G) a == Some ([::], L).
-      {
-        case: (project G a)=>/=// L' /(_ L').
-        rewrite eq_refl=>/(_ is_true_true) =>/eqP->.
-        case: P=>//; first (by case: (project_all G ps)).
-        move=> lG P; move: (Ih P); case: (project_all G ps) =>// P' {Ih}H.
-        by move=>/eqP-[-> PP']; move: PP' H =>-> /(_ (eq_refl _))->/=.
-      }
-      move=> {Ih P ps}.
-      elim/gty_ind2: G=>//.
-      + move=> G Ih L/=; move: Ih.
-        case: (project G a)=>// L' /(_ L' (eq_refl _))/eqP->/=.
-        by rewrite -[Some _ == Some _]/(L' == _); case: ifP.
-      + move=> [[p q] ty] G/=; rewrite /ml_send/ml_recv.
-        case: (ifP (p == q))=>//.
-        case: (project G a) =>//;
-          last (by case: (ifP (p == a))=>//; case: (ifP (q == a))).
-        move=>L _ /(_ L (eq_refl _)) /eqP-> L'/=.
-        by (do ! case: ifP=>//).
-      + move=> [[p q] ty] K Ih/= L.
-  Admitted. (* TODO: Fix q_proj to simplify proof *)
+      rewrite /q_proj msg_project_init rg_project_init option_comm.
+      case: (project G a)=>// L.
+      by move: Ih; case: (project_all G ps) =>// K /(_ K (eq_refl _))-> /eqP-[->].
+  Qed.
 
   Theorem global_local_trequiv G :
     forall P,
